```agda
{-# OPTIONS --without-K #-}
open import prelude hiding (_∘_ ; _×_ ; Σ)

module ch01 where
```

# Exercise 1.1.

Given functions $f : A → B$ and $g : B → C$, define their composition $g ∘ f : A → C$. Show that $f ∘ (g ∘ h) ≡ (f ∘ g) ∘ h$.
```agda
  _∘_ : {A B C : Type} → (g : B → C) → (f : A → B) → A → C
  (g ∘ f) a = g (f a)

  ∘-assoc : {A B C D : Type} → (f : C → D) → (g : B → C) → (h : A → B) → f ∘ (g ∘ h) ≡ (f ∘ g) ∘ h
  ∘-assoc f g h = refl (λ x → f (g (h x)))
```

# Exercise 1.2.

Derive the recursion principle for products using only the projections, and verify that the definitional equalities are valid. Do the same for Σ types.

```agda
  data _×_ (A B : Type) : Type where
    _,_ : A → B → A × B

  ×-rec : {A B C : Type} →
        (A → B → C) →
        A × B → C
  ×-rec f (a , b) = f a b

  π₁ : {A B : Type} → A × B → A
  π₁ (a , _) = a

  π₂ : {A B : Type} → A × B → B
  π₂ (_ , b) = b

  ×-rec-again : {A B C : Type} →
              (A → B → C) →
              A × B → C
  ×-rec-again f p = f (π₁ p) (π₂ p)
```

We see that `π₁ p :≡ a` and that `π₂ p :≡ b`. Thus, `×-rec-again` satisfies the required definitional equality.

```agda
  data Σ (A : Type) (B : A → Type) : Type where
    _,_ : (a : A) → (y : B a) → Σ A B

  Σ-rec : {A : Type} {B : A → Type} {C : Type} →
        ((a : A) → B a → C) →
        Σ A B → C
  Σ-rec f (a , b) = f a b

  Σπ₁ : {A : Type} {B : A → Type} → Σ A B → A
  Σπ₁ (a , _) = a

  Σπ₂ : {A : Type} {B : A → Type} → (p : Σ A B) → B (Σπ₁ p)
  Σπ₂ (_ , b) = b

  Σ-rec-again : {A : Type} {B : A → Type} {C : Type} →
              ((a : A) → B a → C) →
              Σ A B → C
  Σ-rec-again f p = f (Σπ₁ p) (Σπ₂ p)
```

Again, we see that `Σπ₁ p :≡ a` and `Σπ₂ p :≡ b`. Thus, `Σ-rec-again` satisfies the required definitional equality.

# Exercise 1.3.

Derive the induction principle for products, using only the projections and the propositional uniqueness principle.

```agda
  tr : {X : Type} {F : X → Type} {x y : X} → x ≡ y → F x → F y
  tr (refl _) = λ z → z

  ×-uniq : {A B : Type} →
         (p : A × B) → (π₁ p , π₂ p) ≡ p
  ×-uniq (a , b) = refl (a , b)

  ×-ind : {A B : Type} {C : A × B → Type} →
        ((a : A) → (b : B) → C (a , b)) →
        (p : A × B) → C p
  ×-ind {A} {B} {C} f p = tr {A × B} {C} {(π₁ p , π₂ p)} {p} (×-uniq p) (f (π₁ p) (π₂ p))

  Σ-uniq : {A : Type} {B : A → Type} →
         (p : Σ A B) → (Σπ₁ p , Σπ₂ p) ≡ p
  Σ-uniq (a , b) = refl (a , b)

  Σ-ind : {A : Type} {B : A → Type} {C : Σ A B → Type} →
        ((a : A) → (b : B a) → C (a , b)) →
        (p : Σ A B) → C p
  Σ-ind {A} {B} {C} f p = tr {Σ A B} {C} {(Σπ₁ p , Σπ₂ p)} {p} (Σ-uniq p) (f (Σπ₁ p) (Σπ₂ p))
```

# Exercise 1.4.

Use the iterator for ℕ to derive a function having the type of the recursor for ℕ. Show that the defining equations for the recursor hold propositionally for this function.
```agda
  ℕ-iter : {C : Type} →
         C → (C → C) → ℕ → C
  ℕ-iter c f zero = c
  ℕ-iter c f (suc n) = f (ℕ-iter c f n)

  ℕ-rec : {C : Type} →
        C → (ℕ → C → C) →
        ℕ → C
  ℕ-rec c f zero = c
  ℕ-rec c f (suc n) = f n (ℕ-rec c f n)

  ℕ-ind : {C : ℕ → Type} →
        C zero →
        ((n : ℕ) → C n → C (suc n)) →
        (n : ℕ) → C n
  ℕ-ind c f zero = c
  ℕ-ind c f (suc n) = f n (ℕ-ind c f n)

  ℕ-fun : {C : Type} →
        C → (ℕ → C → C) →
        ℕ → C
  ℕ-fun c f n = π₂ (ℕ-iter (zero , c) (λ p → (suc (π₁ p) , f (π₁ p) (π₂ p))) n)

  ℕ-fun-zero : {C : Type} → (c : C) → (f : ℕ → C → C) →
             ℕ-fun c f zero ≡ c
  ℕ-fun-zero c f = refl c

  ℕ-fun-suc : {C : Type} → (c : C) (f : ℕ → C → C) (n : ℕ) →
            ℕ-fun c f (suc n) ≡ f n (ℕ-rec c f n)
  ℕ-fun-suc c f = ℕ-ind (refl (f zero c)) λ n eq → ap₂ f (lma₁ (suc n)) (ap₂ f (lma₁ n) (lma₂ n)) where
    lma₁ : (n : ℕ) → π₁ (ℕ-iter (zero , c) (λ p → suc (π₁ p) , f (π₁ p) (π₂ p)) n) ≡ n
    lma₁ = ℕ-ind (refl zero) λ n eq → ap suc eq

    lma₂ : (n : ℕ) → π₂ (ℕ-iter (zero , c) (λ p → suc (π₁ p) , f (π₁ p) (π₂ p)) n) ≡ ℕ-rec c f n
    lma₂ = ℕ-ind (refl c) λ n eq → ap₂ f (lma₁ n) eq
```

# Exercise 1.5.

Show that if we define `A ∔ B :≡ Σ (x : 𝟚) (𝟚-rec A B x)`, then we can give a definition of `∔-ind` for which the definitional equalities stated in §1.7 hold.
```agda
  data 𝟚 : Type where
    𝟎 𝟏 : 𝟚

  𝟚-rec : {i : Level} {C : Type i} → C → C → 𝟚 → C
  𝟚-rec c₀ c₁ 𝟎 = c₀
  𝟚-rec c₀ c₁ 𝟏 = c₁

  module _ where private
    _∔_ : Type → Type → Type
    A ∔ B = Σ 𝟚 (λ (x : 𝟚) → 𝟚-rec A B x)

    ∔-ind : {A B : Type} {C : A ∔ B → Type} →
          ((a : A) → C (𝟎 , a)) →
          ((b : B) → C (𝟏 , b)) →
          (b : A ∔ B) → C b
    ∔-ind f g (𝟎 , a) = f a
    ∔-ind f g (𝟏 , b) = g b
```

`(𝟎 , a)` encodes `inl(a)` and `(𝟏 , b)` encodes `inr(b)`. We see that `∔-ind` satisfies the required definitional equalities.

# Exercise 1.9.

Define the type family `Fin : ℕ → 𝓤` mentioned at the end of §1.3, and the dependent function `fmax : Π (n : ℕ) Fin(suc n)` mentioned in §1.4.
```agda
  data 𝟘 : Type where

  data _∔_ (A B : Type) : Type where
    inl : A → A ∔ B
    inr : B → A ∔ B
    
  Fin : ℕ → Type
  Fin zero = 𝟘
  Fin (suc n) = (Fin n) ∔ 𝟙

  fmax : (n : ℕ) → Fin (suc n)
  fmax n = inr ⋆
```

# Exercise 1.10.

Show that the Ackermann function `ack : ℕ → ℕ → ℕ` is definable using only `ℕ-rec` satisfying the following equations:
- `ack 0 n :≡ suc n`
- `ack (suc m) 0 :≡ ack m 1`
- `ack (suc m) (suc n) :≡ ack m (ack (suc m) n)`

```agda
  ack : ℕ → ℕ → ℕ
  ack = ℕ-rec (λ n → suc n) (λ m f → ℕ-rec (f (suc zero)) (λ n r → f r))
```

We can check that the definitional equalities are satisfied:
- ℕ-rec (λ n → suc n) (λ m f → ℕ-rec (f (suc zero)) (λ n r → f r)) 0 n  
    = (λ n → suc n) n  
    = suc n

- ℕ-rec (λ n → suc n) (λ m f → ℕ-rec (f (suc zero)) (λ n r → f r)) (suc m) 0  
    = (λ m f → ℕ-rec (f (suc zero)) (λ n r → f r)) m (ℕ-rec (λ n → suc n) (λ m f → ℕ-rec (f (suc zero)) (λ n r → f r)) m) 0  
    = (λ f → ℕ-rec (f (suc zero)) (λ n r → f r)) (ℕ-rec (λ n → suc n) (λ m f → ℕ-rec (f (suc zero)) (λ n r → f r)) m) 0  
    = ℕ-rec ((ℕ-rec (λ n → suc n) (λ m f → ℕ-rec (f (suc zero)) (λ n r → f r)) m) (suc zero)) (λ n r → (ℕ-rec (λ n → suc n) (λ m f → ℕ-rec (f (suc zero)) (λ n r → f r)) m) r) 0  
    = (ℕ-rec (λ n → suc n) (λ m f → ℕ-rec (f (suc zero)) (λ n r → f r)) m) (suc zero)  
    = ack m 1

- ℕ-rec (λ n → suc n) (λ m f → ℕ-rec (f (suc zero)) (λ n r → f r)) 1 1  
          :≡ (λ m f → ℕ-rec (f (suc zero)) (λ n r → f r)) 0 (ℕ-rec (λ n → suc n) (λ m f → ℕ-rec (f (suc zero)) (λ n r → f r)) 0) 1  
          :≡ (λ f → ℕ-rec (f (suc zero)) (λ n r → f r)) (ℕ-rec (λ n → suc n) (λ m f → ℕ-rec (f (suc zero)) (λ n r → f r)) 0) 1  
          :≡ (λ f → ℕ-rec (f (suc zero)) (λ n r → f r)) (λ n → suc n) 1  
          :≡ ℕ-rec ((λ n → suc n) (suc zero)) (λ n r → (λ n → suc n) r) 1  
          :≡ ℕ-rec (suc (suc zero)) (λ n r → suc r) 1  
          :≡ (λ n r → suc r) 0 (ℕ-rec (suc (suc zero)) (λ n r → suc r) 0)  
          :≡ (λ r → suc r) (suc (suc zero))  
  ack 1 1 :≡ suc (suc (suc zero))
